Cslib/Foundations/Semantics/LTS/Reverse.lean
@@ -1,0 +1,53 @@
+/-
+Copyright (c) 2026 Vignesh Karri. All rights reserved.
+Released under Apache 2.0 license as described in the file LICENSE.
+Authors: Vignesh Karri
+-/
+
+module
+
+public import Cslib.Foundations.Semantics.LTS.Basic
+
+/-!
+# Reverse operation for LTS.
+-/
+
+@[expose] public section
+
+namespace Cslib.LTS
+
+section Reverse
+
+/-- Constructs an LTS by reversing the transitions of an existing LTS. -/
+def reverse (lts : LTS State Label) : LTS State Label where
+  Tr s μ s' := lts.Tr s' μ s
+
+@[simp]
+theorem reverse_tr {lts : LTS State Label} :
+    (lts.reverse).Tr s μ s' ↔ lts.Tr s' μ s := by rfl
+
+/-- Reversing an LTS twice gives back the original LTS. -/
+@[simp]
+theorem reverse_reverse (lts : LTS State Label) : lts.reverse.reverse = lts := rfl
+
+/-- The multistep transitions of `lts.reverse` are exactly the reversed multistep transitions of
+`lts` -/
+@[simp]
+theorem reverse_mTr {lts : LTS State Label} :
+    lts.reverse.MTr s' μs s ↔ lts.MTr s μs.reverse s' := by
+  induction μs generalizing s s' with
+  | nil =>
+    simp_all [eq_comm]
+  | cons x xs ih =>
+    simp only [List.reverse_cons, LTS.MTr.cons_iff]
+    constructor
+    · rintro ⟨mid, h1, h2⟩
+      exact LTS.MTr.stepR lts (ih.mp h2) h1
+    · intro hmtr
+      obtain ⟨mid, h1, h2⟩ := LTS.MTr.split hmtr
+      simp only [LTS.MTr.singleton_iff] at h2
+      exact ⟨mid, h2, ih.mpr h1⟩
+
+end Reverse
+
+end Cslib.LTS
